Finalized report, and files accordingly

coq/Main.v
@@ -15,7 +15,7 @@ Open Scope nat_scope.
 Import ListNotations.
 
 Definition build (xs : list tree) (P : xs <> []) : tree := 
-  foldl1 join (fold_right (fun (a : tree) (xs : list tree) => step a xs (length xs)) nil xs) (fold_step_not_nil xs P).
+  foldl1 join (fold_right (fun (a : tree) (xs : list tree) => step a xs) nil xs) (fold_step_not_nil xs P).
 
 Theorem build_is_min : forall (l : list tree) (t : tree) (P : l <> nil), 
   t = build l P -> minimum l t.
@@ -23,3 +23,6 @@ Proof.
   intros l t NNil BRes. unfold build in BRes. rewrite BRes. apply foldl1_is_min. 
     reflexivity.
 Qed.
+
+(* The example from the paper, which outputs the same result *)
+Eval compute in build [Tip 4; Tip 2; Tip 3; Tip 5; Tip 1; Tip 4; Tip 6].
