coq/StepN.v
@@ -1,0 +1,79 @@
+
+Require Import Coq.Strings.String.
+Require Import Coq.Lists.List.
+Require Import Coq.Arith.Compare_dec.
+Require Import Coq.Arith.Lt.
+Require Import Coq.Arith.Gt.
+Require Import Arith.Wf_nat.
+Require Import Helpers.
+Require Import Recdef.
+Require Import Tree.
+
+Open Scope nat_scope.
+
+Import ListNotations.
+
+Fixpoint step (t : tree) (xs : list tree) (n : nat) {struct n} : list tree :=
+  match n with
+  | 0 => [t]
+  | S n2 =>
+    match xs with
+    | nil      => [t]
+    | u :: nil =>
+        match nat_compare (ht t) (ht u) with
+        | Lt => t :: u :: nil
+        | _  => (join t u) :: nil
+        end
+    | u :: v :: ts =>
+        match nat_compare (ht t) (ht u) with
+        | Lt => t :: u :: v :: ts
+        | _  =>
+            match nat_compare (ht t) (ht v) with
+            | Lt => step (join t u) (v :: ts) (n2)
+            | _  => step t (step (join u v) ts n2) (n2)
+            end
+        end
+    end
+  end.
+
+Theorem step_not_nil : forall (ts : list tree) (t : tree),
+  step t ts (length ts) <> [].
+Proof.
+  intros ts.
+  (* match n *)  induction (length ts) as [|n2]. 
+  (* | 0 => [t] *) simpl. intuition. inversion H.
+  (* | S n2 => *) 
+    (* match xs *) induction ts as [|u].
+    (* | nil      => [t] *)  simpl. intuition. inversion H. 
+    (* | u :: nil => *) induction ts as [|v].
+        (* match nat_compare (ht t) (ht u) with *) intros t. remember (nat_compare (ht t) (ht u)) as R1. induction R1. 
+        (* | Eq => (join t u) :: nil *) simpl. rewrite <- HeqR1. intuition. inversion H.
+        (* | Lt => t :: u :: nil *) simpl. rewrite <- HeqR1. intuition. inversion H.
+        (* | Gt => (join t u) :: nil *) simpl. rewrite <- HeqR1. intuition. inversion H.
+        (* end *)
+   (* | u :: v :: ts => *)
+        (* match nat_compare (ht t) (ht u) with *) intros t. remember (nat_compare (ht t) (ht u)) as R2. induction R2.
+        (* | Eq => *)
+            (* match nat_compare (ht t) (ht v) with *) remember (nat_compare (ht t) (ht v)) as R3. induction R3.
+            (* | Eq => step t (step (join u v) ts n2) (n2) *) simpl. rewrite <- HeqR2. rewrite <- HeqR3.
+            (* | Lt => step (join t u) (v :: ts) (n2) *)
+            (* | Gt => step t (step (join u v) ts n2) (n2) *)
+            (* end *)
+        (* | Lt => t :: u :: v :: ts *)
+        (* | Gt => *)
+            (* match nat_compare (ht t) (ht v) with *)
+            (* | Lt => step (join t u) (v :: ts) (n2) *)
+            (* | _  => step t (step (join u v) ts n2) (n2) *)
+            (* end *)
+        (* end *)
+    (* end *)
+  (* end. *)
+Admitted.
+
+Theorem step_join_le : forall (l : list tree) (t u : tree) (n : nat) (P : n >= length l),
+  length (step (join t u) l n) <= length (u :: l).
+Proof.
+  induction n. intros Len. simpl. intuition.
+
+  induction l. simpl. intuition.
+    simpl. remember (nat_compare (max (ht t) 
